wjirbgijere

Games/gameLib_fixfix/Stealing.lean
@@ -12,12 +12,15 @@ import Games.gameLib_fixfix.Zermelo
 
 structure Bait (g : zSymm_Game_World α β) (trap : β) : Prop where
   leg_fst : g.law g.init_game_state [] trap
-  leg_imp : ∀ hist, ∀ act, g.law g.init_game_state (hist ++ [trap]) act → g.law g.init_game_state (hist) act
-  leg_imp' : ∀ hist, ∀ act, (Z : ¬ hist = []) → hist.getLast Z = trap → Turn_fst (hist.length + 1) → g.law g.init_game_state hist.dropLast act → g.law g.init_game_state hist act
-  leg_hist : ∀ hist, Hist_legal g.init_game_state g.law g.law (hist ++ [trap])  → Hist_legal g.init_game_state g.law g.law (hist)
+  leg_imp : ∀ hist, ∀ act, Hist_legal g.init_game_state g.law g.law (hist) → g.law g.init_game_state (hist ++ [trap]) act → g.law g.init_game_state (hist) act
+  leg_imp' : ∀ hist, ∀ act, Hist_legal g.init_game_state g.law g.law (hist) → (Z : ¬ hist = []) → hist.getLast Z = trap → Turn_fst (hist.length + 1) → g.law g.init_game_state hist.dropLast act → g.law g.init_game_state hist act
+  leg_hist : ∀ hist, Hist_legal g.init_game_state g.law g.law (hist ++ [trap]) → Hist_legal g.init_game_state g.law g.law (hist)
 
 
+-- TODO: leg_hist sounds like it can be derived from leg_imp
 
+
+-- replace by legality if snd condition unnessecary
 structure hist_match_sStrat (g : zSymm_Game_World α β) (ws : sStrategy g.init_game_state g.law g.law) (hist : List β) : Prop where
   leg : Hist_legal g.init_game_state g.law g.law hist
   --coin : ∀ t, (tl : t < hist.length) → (T : Turn_snd (t+1)) → hist.rget ⟨t, tl⟩ = ws (hist.rtake t) (by rw [List.length_rtake (le_of_lt tl)] ; exact T) (Hist_legal_rtake g.init_game_state g.law g.law hist t leg)
@@ -31,7 +34,7 @@ def stolen_strat (g : zSymm_Game_World α β)
   (trap : β) (hb : Bait g trap) (ws : sStrategy g.init_game_state g.law g.law) : fStrategy g.init_game_state g.law g.law :=
   fun h ht hl =>  if M : hist_match_sStrat g ws (h ++ [trap])
                   then  let move := (ws (h ++ [trap]) (by rw [List.length_append, List.length_singleton, ← Turn_fst_snd_step] ; exact ht) M.leg)
-                        ⟨move.val, hb.leg_imp h move.val (move.prop)⟩
+                        ⟨move.val, hb.leg_imp h move.val hl (move.prop)⟩
                   else g.exStrat_fst g.hgp h ht hl
 
 noncomputable
@@ -41,19 +44,20 @@ def pre_stolen_strat (g : zSymm_Game_World α β)
                   then ⟨trap, (by rw [Z] ; exact hb.leg_fst)⟩
                   else  if M : h.getLast Z = trap
                         then  let move := s_strat h.dropLast (by rw [List.length_dropLast, Nat.sub_add_cancel, Turn_snd_fst_step] ; exact ht ; rw [Nat.succ_le, List.length_pos] ; exact Z) (by have := List.dropLast_append_getLast Z ; rw [M] at this ; apply hb.leg_hist ; rw [this] ; exact hl)
-                              ⟨move.val, hb.leg_imp' h move.val Z M ht move.prop⟩
+                              ⟨move.val, hb.leg_imp' h move.val hl Z M ht move.prop⟩
                         else  g.exStrat_fst g.hgp h ht hl
 
 
 
 
-
-#exit
+--#exit
 
 structure Stealing_condition (g : zSymm_Game_World α β) where
   trap : β
   hb : Bait g trap
-  wb : ∀ hist, Hist_legal g.init_game_state g.law g.law hist → (g.fst_win_states g.init_game_state (hist ++ [trap]) ↔ g.fst_win_states g.init_game_state hist)
+  fst_not_win : ¬ g.snd_win_states g.init_game_state []
+  wb : ∀ hist, Hist_legal g.init_game_state g.law g.law hist → (g.snd_win_states g.init_game_state (hist ++ [trap]) ↔ g.fst_win_states g.init_game_state hist)
+
 
 theorem Strategy_stealing (g : zSymm_Game_World α β) (s : Stealing_condition g) : g.is_fst_win :=
   by
@@ -63,8 +67,28 @@ theorem Strategy_stealing (g : zSymm_Game_World α β) (s : Stealing_condition g
     let sto_strat := stolen_strat g s.trap s.hb ws
     use sto_strat
     intro s_strat
+    let pre_sto_strat := pre_stolen_strat g s.trap s.hb s_strat
+    specialize ws_prop pre_sto_strat
+    obtain ⟨T,Tw,Tn⟩ := ws_prop
+    apply Game.coherent_end_fst_win _ (by apply g.hgn)
+    cases' T with T
+    · dsimp [History_on_turn] at Tw
+      exfalso
+      exact s.fst_not_win Tw
+    · use T
+      dsimp at Tw Tn
+      dsimp
+      sorry
 
 
+/-
+Show :
+History_on_turn g.init_game_state g.law g.law (pre_stolen_strat g s.trap (_ : Bait g s.trap) s_strat) ws (Nat.succ T) =
+(History_on_turn g.init_game_state g.law g.law (stolen_strat g s.trap (_ : Bait g s.trap) ws) s_strat T)) ++ [trap]
+
+Then use s.wb to conclude
+
+-/
 
 
 
